refactor: Modify the Airlock example to be easier to reason with
Our main goal with this modification is to be able to reason about the
airlock program trustworthiness without the need to explore manually
the case where we open one door or the other.

core/examples/airlock.v
@@ -23,29 +23,29 @@ From FreeSpec Require Import Core.
 
 (** * Specifying
 
-    ** Door *)
+    ** Doors *)
 
-Inductive DOOR {l} (d : l) : interface :=
-| IsOpen : DOOR d bool
-| Toggle : DOOR d unit.
+Inductive door : Type := left | right.
 
-Definition is_open {ix l} (d : l) `{ix :| DOOR d} : program ix bool :=
+Inductive DOORS : interface :=
+| IsOpen : door -> DOORS bool
+| Toggle : door -> DOORS unit.
+
+Definition is_open {ix} `{ix :| DOORS} (d : door) : program ix bool :=
   request (IsOpen d).
 
-Definition toggle {ix l} (d : l) `{ix :| DOOR d} : program ix unit :=
+Definition toggle {ix} `{ix :| DOORS} (d : door) : program ix unit :=
   request (Toggle d).
 
-Definition open_door {ix l} (d : l) `{ix :| DOOR d} : program ix unit :=
+Definition open_door {ix} `{ix :| DOORS} (d : door) : program ix unit :=
   var open ← is_open d in
   when (negb open) (toggle d).
 
-Definition close_door {ix l} (d : l) `{ix :| DOOR d} : program ix unit :=
+Definition close_door {ix} `{ix :| DOORS} (d : door) : program ix unit :=
   var open ← is_open d in
   when open (toggle d).
 
 (** ** Controller *)
-
-Inductive door : Type := left | right.
 
 Inductive CONTROLLER : interface :=
 | Tick : CONTROLLER unit
@@ -63,27 +63,132 @@ Definition co (d : door) : door :=
   | right => left
   end.
 
-Instance door_Provide (d : door) : Provide (DOOR left ⊕ DOOR right) (DOOR d) :=
-  { lift_eff := match d with
-                | left => fun _ op => in_left op
-                | right => fun _ op => in_right op
-                end
-  }.
-
 From Prelude Require Import State.
 
-Definition controller : component CONTROLLER (DOOR left ⊕ DOOR right) nat :=
+Definition controller : component CONTROLLER DOORS nat :=
   fun _ op =>
     match op with
     | Tick =>
       var cpt ← get in
-      when (15 <? cpt) $ do lift (close_door left);
-                            lift (close_door right);
-                            put 0
-    | RequestOpen d =>
-      do lift (close_door (co d));
-         lift (open_door d);
-         put 0
+      when (15 <? cpt) (do
+        lift (close_door left);
+        lift (close_door right);
+        put 0)
+    | RequestOpen d => do
+        lift (close_door (co d));
+        lift (open_door d);
+        put 0
     end.
 
 (** * Verifying *)
+
+Definition Ω : Type := bool * bool.
+
+Definition sel (d : door) : Ω -> bool :=
+  match d with
+  | left => fst
+  | right => snd
+  end.
+
+Definition tog (d : door) (ω : Ω) : Ω :=
+  match d, ω with
+  | left, (l, r) => (negb l, r)
+  | right, (l, r) => (l, negb r)
+  end.
+
+Lemma tog_equ_1 (d : door) (ω : Ω)
+  : sel d (tog d ω) = negb (sel d ω).
+Proof.
+  destruct d; destruct ω; reflexivity.
+Qed.
+
+Lemma tog_equ_2 (d : door) (ω : Ω)
+  : sel (co d) (tog d ω) = sel (co d) ω.
+Proof.
+  destruct d; destruct ω; reflexivity.
+Qed.
+
+Opaque tog.
+
+Definition step (a : Type) (ω : Ω) (e : DOORS a) (x : a) :=
+  match e with
+  | Toggle d => tog d ω
+  | _ => ω
+  end.
+
+Inductive req : forall (a : Type), Ω -> DOORS a -> Prop :=
+| req_is_open (d : door) (ω : Ω)
+  : req bool ω (IsOpen d)
+
+| req_toggle (ω : Ω) (d : door) (H : sel d ω = false -> sel (co d) ω = false)
+  : req unit ω (Toggle d).
+
+Inductive prom: forall (a : Type), Ω -> DOORS a -> a -> Prop :=
+
+| prom_is_open (d : door) (ω : Ω) (x : bool) (equ : sel d ω = x)
+  : prom bool ω (IsOpen d) x
+
+| prom_toggle (d : door)(ω : Ω) (x : unit)
+  : prom unit ω (Toggle d) x.
+
+Definition doors_specs : specs DOORS Ω :=
+  {| witness_update := step
+  ; requirements := req
+  ; promises := prom
+  |}.
+
+From Prelude Require Import Tactics.
+
+Lemma close_door_trustworthy (ω : Ω) (d : door)
+  : trustworthy_program doors_specs ω (close_door d).
+
+Proof.
+  prove_program; cbn; repeat constructor; subst.
+  inversion Hpost; ssubst.
+  now rewrite H1.
+Qed.
+
+Lemma open_door_trustworthy (ω : Ω) (d : door) (safe : sel (co d) ω = false)
+  : trustworthy_program doors_specs ω (open_door d).
+
+Proof.
+  prove_program; cbn; repeat constructor; subst.
+  inversion Hpost; ssubst.
+  now rewrite safe.
+Qed.
+
+Definition safe_open_door {ix} `{ix :| DOORS} (d : door) : program ix unit :=
+  do close_door (co d);
+     open_door d.
+
+Lemma close_door_run (ω : Ω) (d : door) (ω' : Ω) (x : unit)
+  (run : trustworthy_run doors_specs (close_door d) ω ω' x)
+  : sel d ω' = false.
+Proof.
+  inversion run; ssubst.
+  cbn in *.
+  inversion prom0; ssubst.
+  case_eq (sel d ω); intros equ; rewrite equ in rec.
+  + inversion rec; ssubst.
+    cbn in rec0.
+    inversion rec0; ssubst.
+    rewrite tog_equ_1.
+    rewrite equ.
+    reflexivity.
+  + inversion rec; ssubst.
+    exact equ.
+Qed.
+
+#[local] Opaque close_door.
+#[local] Opaque open_door.
+
+Lemma safe_door_trustworthy (ω : Ω) (d : door)
+  : trustworthy_program doors_specs ω (safe_open_door d).
+
+Proof.
+  prove_program; cbn; repeat constructor; subst.
+  apply close_door_trustworthy.
+  apply close_door_run in Hrun.
+  apply open_door_trustworthy.
+  exact Hrun.
+Qed.
